Checkpoint more fixes

new/golang/defn/postlang.v
@@ -5,6 +5,33 @@
 From Perennial.goose_lang Require Export lang notation.
 From Perennial Require Export base.
 
+(** [GoContext] contains several low-level Go functions for typed memory access,
+    map updates, etc. *)
+Class GoContext {ext : ffi_syntax} : Type :=
+  {
+    global_addr : go_string → loc;
+    functions : go_string → list go.type → val;
+    methods : go.type → go_string → val;
+
+    alloc : go.type → val;
+    load : go.type → val;
+    store : go.type → val;
+
+    struct_field_ref : go.type → go_string → loc → loc;
+
+    index (container_type : go.type) (i : Z) (v : val) : expr;
+    index_ref (container_type : go.type) (i : Z) (v : val) : expr;
+    array_index_ref (elem_type : go.type) (i : Z) (l : loc) : loc;
+
+    to_underlying : go.type → go.type;
+    is_map_pure (v : val) (m : val → bool * val) : Prop;
+    map_lookup : val → val → bool * val;
+    map_insert : val → val → val → val;
+  }.
+
+Definition slice_index_ref `{GoContext} (elem_type : go.type) (i : Z) (s : slice.t) : loc :=
+  array_index_ref elem_type i s.(slice.ptr).
+
 Class IntoVal {ext : ffi_syntax} (V : Type) :=
   {
     to_val_def : V → val;
@@ -44,7 +71,7 @@ Section goose_lang.
 Context `{ffi_syntax}.
 
 Inductive t :=
-| mk (type_id : go_string) (v : val) : t
+| mk (ty : go.type) (v : val) : t
 | nil : t.
 
 End goose_lang.
@@ -107,8 +134,8 @@ Global Instance into_val_interface : IntoVal interface.t :=
   {|
     to_val_def (i: interface.t) :=
       match i with
-      | interface.nil => NONEV
-      | interface.mk type_id v => SOMEV (#type_id, v)%V
+      | interface.nil => InterfaceV None
+      | interface.mk ty v => InterfaceV $ Some (ty, v)
       end;
     zero_val := interface.nil;
   |}.
@@ -139,8 +166,20 @@ Definition bool : go.type := go.Named "bool"%go [].
 Definition byte : go.type := uint8.
 Definition rune : go.type := uint32.
 
+(* built-in functions *)
+Definition make3 : go_string := "make3".
+Definition make2 : go_string := "make2".
+Definition len : go_string := "len".
+Definition cap : go_string := "cap".
+
 Section defs.
 Context `{ffi_syntax}.
+
+(* helpers for signed comparisons *)
+Definition int_lt : val := λ: "x" "y", BinOp SignedLtOp "x" "y".
+Definition int_leq : val := λ: "x" "y", BinOp SignedLeOp "x" "y".
+Definition int_geq : val := λ: "x" "y", int_leq "y" "x".
+Definition int_gt : val := λ: "x" "y", int_lt "y" "x".
 
 Inductive is_primitive : go.type → Prop :=
 | is_primitive_uint64 : is_primitive uint64
@@ -181,8 +220,56 @@ Inductive is_primitive_zero_val : go.type → ∀ {V} `{!IntoVal V}, V → Prop 
 | is_primitive_zero_val_channel dir t : is_primitive_zero_val (go.ChannelType dir t) null
 .
 
-(** [go.ContextValid] defines when a GoContext is valid. *)
-Class ContextValid `{!GoContext} :=
+Inductive is_go_step_pure `{!GoContext} :
+  ∀ (op : go_op) (arg : val) (e' : expr), Prop :=
+| angelic_exit_step : is_go_step_pure AngelicExit #() (GoInstruction AngelicExit #())%E
+| load_step t arg : is_go_step_pure (GoLoad t) arg (load t arg)
+| store_step t arg : is_go_step_pure (GoStore t) arg (store t arg)
+| alloc_step t : is_go_step_pure (GoAlloc t) #() (alloc t #())%E
+| prealloc_step (l : loc) : is_go_step_pure GoPrealloc #() #l
+| func_call_step f targs : is_go_step_pure (FuncCall f targs) #() (functions f targs)
+| method_call_step t m : is_go_step_pure (MethodCall t m) #() (methods t m)
+| global_var_addr_step v : is_go_step_pure (GlobalVarAddr v) #() #(global_addr v)
+| struct_field_ref_step t f l : is_go_step_pure (StructFieldRef t f) #l #(struct_field_ref t f l)
+| struct_field_get_step f m v (Hf : m !! f = Some v) :
+  is_go_step_pure (StructFieldGet f) (StructV m) (Val v)
+| struct_field_set_step f m v :
+  is_go_step_pure (StructFieldSet f) (StructV m, v)%V (StructV $ <[ f := v ]> m)
+
+| internal_len_slice_step_pure elem_type s :
+  is_go_step_pure (InternalLen (go.SliceType elem_type)) #s #s.(slice.len)
+| internal_len_array_step_pure elem_type n v :
+  is_go_step_pure (InternalLen (go.ArrayType n elem_type)) v #(W64 n)
+
+| internal_cap_slice_step_pure elem_type s :
+  is_go_step_pure (InternalCap (go.SliceType elem_type)) #s #s.(slice.cap)
+| internal_dynamic_array_alloc_pure elem_type (n : w64) :
+  is_go_step_pure (InternalDynamicArrayAlloc elem_type) #n
+    (GoInstruction (GoAlloc $ go.ArrayType (sint.Z n) elem_type) #())
+| internal_slice_make_pure p l c :
+  is_go_step_pure InternalMakeSlice (#p, #l, #c) #(slice.mk p l c)
+| slice_array_step_pure n elem_type p l c :
+  is_go_step_pure (Slice (go.ArrayType n elem_type)) (#p, (#l, #c))%V #(slice.mk p l c)
+| index_ref_step t v (j : w64) : is_go_step_pure (IndexRef t) (v, #j) (index_ref t (sint.Z j) v)
+| index_step t v (j : w64) : is_go_step_pure (Index t) (v, #j) (index t (sint.Z j) v)
+| array_append_step_pure l v : is_go_step_pure ArrayAppend (ArrayV l) (ArrayV $ l ++ [v])
+| internal_map_lookup_step_pure m k :
+  is_go_step_pure InternalMapLookup (m, k) (let '(ok, v) := map_lookup m k in (v, #ok))
+| internal_map_insert_step_pure m k v :
+  is_go_step_pure InternalMapLookup (m, k, v) (map_insert m k v)
+.
+
+(* TODO: add requirement that goose_go_stepper = this thing *)
+Inductive is_go_step `{!GoContext} :
+  ∀ (op : go_op) (arg : val) (e' : expr) (s : gset go_string) (s' : gset go_string), Prop :=
+| go_step_pure op arg e' (Hpure : is_go_step_pure op arg e') s : is_go_step op arg e' s s
+| package_init_check_step s p : is_go_step (PackageInitCheck p) #() #(bool_decide (p ∈ s)) s s
+| package_init_mark_step s p : is_go_step (PackageInitMark p) #() #() s (s ∪ {[p]})
+.
+
+(** [go.ValidCore] defines when a GoContext is valid, excluding slice, map, and
+    channel stuff. *)
+Class ValidCore `{!GoContext} :=
 {
   alloc_underlying t : alloc t = alloc (to_underlying t);
   alloc_primitive t {V} (v : V) `{!IntoVal V} (H : is_primitive_zero_val t v) :
@@ -228,7 +315,7 @@ Class ContextValid `{!GoContext} :=
     (λ: "l",
        foldl (λ array_so_far j,
                 let elem_addr :=
-                  GoInstruction (ArrayIndexRef (go.ArrayType n elem_type)) #(W64 j) "l" in
+                  GoInstruction (IndexRef (go.ArrayType n elem_type)) #(W64 j) "l" in
                 let elem_val := GoInstruction (GoLoad elem_type) elem_addr in
                 GoInstruction ArrayAppend (array_so_far, elem_val)
          )
@@ -257,13 +344,56 @@ Class ContextValid `{!GoContext} :=
        foldl (λ str_so_far j,
                 str_so_far;;
                 let elem_addr :=
-                  GoInstruction (ArrayIndexRef (go.ArrayType n elem_type)) #(W64 j) "l" in
-                let elem_val := GoInstruction ArrayLookup ("v", #(W64 n)) in
+                  GoInstruction (IndexRef (go.ArrayType n elem_type)) #(W64 j) "l" in
+                let elem_val := GoInstruction (Index $ go.ArrayType n elem_type) ("v", #(W64 n)) in
                 GoInstruction (GoStore elem_type) (elem_addr, elem_val))
              (ArrayV []) (seqZ 0 n)
     )%V;
 
   struct_field_ref_underlying t : struct_field_ref t = struct_field_ref (to_underlying t);
+
+  index_ref_underlying t : index_ref t = index_ref (to_underlying t);
+  index_ref_array n elem_type i l :
+    index_ref (go.ArrayType n elem_type) i #l = #(array_index_ref elem_type i l);
+  index_ref_slice elem_type i s (Hrange : 0 ≤ i < sint.Z s.(slice.len)) :
+    index_ref (go.SliceType elem_type) i #s = #(slice_index_ref elem_type i s);
+
+  index_underlying t : index t = index (to_underlying t);
+  index_array n elem_type i l v (Hinrange : l !! (Z.to_nat i) = Some v):
+    index (go.ArrayType n elem_type) i (ArrayV l) = (Val v);
+  index_slice elem_type i (s : slice.t) :
+    index (go.SliceType elem_type) i #s =
+    GoInstruction (GoLoad elem_type) $ GoInstruction (Index $ go.SliceType elem_type) #(W64 i) #s;
+
+  len_underlying t :
+    functions len [t] = functions len [to_underlying t];
+  len_slice elem_type :
+  functions len [go.TypeLit $ go.SliceType elem_type] =
+  (λ: "s", GoInstruction (InternalLen (go.SliceType elem_type)) "s")%V;
+
+  cap_underlying t :
+  functions cap [t] = functions cap [to_underlying t];
+  cap_slice elem_type :
+      functions cap [go.TypeLit $ go.SliceType elem_type] =
+      (λ: "s", GoInstruction (InternalCap (go.SliceType elem_type)) "s")%V;
+
+  make3_underlying t :
+    functions make3 [t] = functions make3 [to_underlying t];
+  make3_slice elem_type :
+    functions make3 [go.TypeLit $ go.SliceType elem_type] =
+    (λ: "t" "len" "cap",
+       if: (int_lt "cap" "len") then Panic "makeslice: cap out of range" else #();;
+       if: (int_lt "len" #(W64 0)) then Panic "makeslice: len out of range" else #();;
+       if: "cap" = #(W64 0) then
+         (* XXX: this computes a nondeterministic unallocated address by using
+            "(Loc 1 0) +ₗ ArbiraryInt"*)
+         GoInstruction InternalMakeSlice (#(Loc 1 0) +ₗ ArbitraryInt, "len", "cap")
+       else
+         let: "p" := GoInstruction (InternalDynamicArrayAlloc elem_type) "cap" in
+         GoInstruction InternalMakeSlice ("p", "len", "cap"))%V;
+  make2_unfold t :
+    functions make2 [t] =
+    (λ: "t" "sz", GoInstruction (FuncCall make3 [t]) #() "t" "sz" "sz")%V;
 }.
 
 End defs.
